Mica/Base.lean
@@ -1,5 +1,6 @@
 -- SUMMARY: Bundle for `Base/`, containing shared utilities.
 
+import Mica.Base.Arity
 import Mica.Base.Fresh
 import Mica.Base.Except
 import Mica.Base.Fixpoint
